Typed arith. expressions, value is NF, step deterministic

Types.v
@@ -2,4 +2,152 @@ Require Export Smallstep.
 
 Hint Constructors multi.
 
+Inductive tm : Type :=
+| ttrue : tm
+| tfalse : tm
+| tif : tm -> tm -> tm -> tm
+| tzero : tm
+| tsucc : tm -> tm
+| tpred : tm -> tm
+| tiszero : tm -> tm.
+
+Inductive bvalue : tm -> Prop :=
+| bv_true : bvalue ttrue
+| bv_false : bvalue tfalse.
+
+Inductive nvalue : tm -> Prop :=
+| nv_zero : nvalue tzero
+| nv_succ : forall t, nvalue t -> nvalue (tsucc t).
+
+Definition value (t:tm) := bvalue t \/ nvalue t.
+
+Hint Constructors bvalue nvalue.
+Hint Unfold value.
+Hint Unfold extend.
+
+Reserved Notation "t1 '==>' t2" (at level 40).
+
+Inductive step : tm -> tm -> Prop :=
+| ST_IfTrue : forall t1 t2,
+        (tif ttrue t1 t2) ==> t1
+| ST_IfFalse : forall t1 t2,
+        (tif tfalse t1 t2) ==> t2
+| ST_If : forall t1 t1' t2 t3,
+        t1 ==> t1' ->
+        (tif t1 t2 t3) ==> (tif t1' t2 t3)
+| ST_Succ : forall t1 t1',
+        t1 ==> t1' ->
+        (tsucc t1) ==> (tsucc t1')
+| ST_PredZero :
+        (tpred tzero) ==> tzero
+| ST_PredSucc : forall t1,
+        nvalue t1 ->
+        (tpred (tsucc t1)) ==> t1
+| ST_Pred : forall t1 t1',
+        t1 ==> t1' ->
+        (tpred t1) ==> (tpred t1')
+| ST_IszeroZero :
+        (tiszero tzero) ==> ttrue
+| ST_IszeroSucc : forall t1,
+        nvalue t1 ->
+        (tiszero (tsucc t1)) ==> tfalse
+| ST_Iszero : forall t1 t1',
+        t1 ==> t1' ->
+        (tiszero t1) ==> (tiszero t1')
+
+where "t1 '==>' t2" := (step t1 t2).
+
+Tactic Notation "step_cases" tactic(first) ident(c) :=
+    first;
+    [ Case_aux c "ST_IfTrue" | Case_aux c "ST_IfFalse"
+    | Case_aux c "ST_If" | Case_aux c "ST_Succ"
+    | Case_aux c "ST_PredZero" | Case_aux c "ST_PredSucc"
+    | Case_aux c "ST_Pred" | Case_aux c "ST_IszeroZero"
+    | Case_aux c "ST_IszeroSucc" | Case_aux c "ST_Iszero" ].
+
+Hint Constructors step.
+
+Notation step_normal_form := (normal_form step).
+
+Definition stuck (t:tm) : Prop :=
+    step_normal_form t /\ ~ value t.
+
+Hint Unfold stuck.
+
+Example some_term_is_stuck :
+    exists t, stuck t.
+Proof.
+    exists (tsucc ttrue).
+    unfold stuck. split.
+    Case "left".
+        unfold normal_form. intro contra.
+        inversion contra. inversion H. inversion H1.
+    Case "right".
+        intro contra. inversion contra.
+        inversion H. inversion H. inversion H1.
+Qed.
+
+Lemma value_is_nf : forall t,
+    value t -> step_normal_form t.
+Proof.
+    unfold normal_form. intros t val contra.
+    destruct val as [Hbval | Hnval].
+    Case "bvalue".
+        induction Hbval;
+            (* solves both ttrue and tfalse *)
+            inversion contra; inversion H.
+    Case "nvalue".
+        induction Hnval;
+            (* solves tzero and prepares tsucc *)
+            inversion contra; inversion H.
+        SCase "tsucc".
+            apply IHHnval. exists t1'. assumption.
+Qed.
+
+Theorem step_deterministic:
+    deterministic step.
+Proof with eauto.
+    unfold deterministic. intros x y1 y2 Hy1 Hy2.
+    generalize dependent y2.
+    step_cases (induction Hy1) Case;
+        intros y2 Hy2; inversion Hy2; subst;
+        try solve [ reflexivity | solve by inversion ].
+    Case "ST_If".
+        rewrite (IHHy1 t1'0). reflexivity. assumption.
+    Case "ST_Succ".
+        rewrite (IHHy1 t1'0). reflexivity. assumption.
+    Case "ST_PredSucc".
+        inversion H1; subst.
+        (* t1 is in NF *)
+        assert (step_normal_form t1) as t1_NF.
+            apply value_is_nf. auto.
+        (* and we cannot step from it any further *)
+        apply ex_falso_quodlibet.
+        apply t1_NF. exists t1'0. assumption.
+    Case "ST_Pred".
+        SCase "1".
+            inversion Hy1; subst.
+            assert (step_normal_form y2) as y2_NF.
+                apply value_is_nf. auto.
+            apply ex_falso_quodlibet.
+            apply y2_NF. exists t1'0. assumption.
+        SCase "2".
+            rewrite (IHHy1 t1'0). reflexivity. assumption.
+    Case "ST_IszeroSucc".
+        SCase "1".
+            inversion H1; subst.
+            assert (step_normal_form t1) as t1_NF.
+                apply value_is_nf. auto.
+            apply ex_falso_quodlibet.
+            apply t1_NF. exists t1'0. assumption.
+        SCase "2".
+            inversion Hy1; subst.
+            assert (step_normal_form t0) as t0_NF.
+                apply value_is_nf. auto.
+            apply ex_falso_quodlibet.
+            apply t0_NF. exists t1'0. assumption.
+        SCase "3".
+            rewrite (IHHy1 t1'0). reflexivity. assumption.
+Qed.
+
 
